complete

compcertox/BQspecx.v
@@ -16,7 +16,7 @@ Inductive bq_internal_state: Type :=
 | bq_init: forall (sig: sig) (vs: list val) (m: mem), bq_internal_state
 | bq_call: forall (sig: RBspec.sig) (vs: list val) (m: mem), bq_internal_state
 | bq_middle: forall (sig: sig) (vs: list val) (m: mem), bq_internal_state
-| bq_middlex: forall (sig: sig) (vs: val) (m: mem), bq_internal_state
+| bq_middle': forall (sig: sig) (vs: val) (m: mem), bq_internal_state
 | bq_final: forall (v: val) (m: mem), bq_internal_state.
 
 Section RB_LTS.
@@ -48,13 +48,13 @@ Section RB_LTS.
   | enq_step2 v1 v2 m:
       bq_step (bq_middle enq [v1; v2] m) E0 (bq_call RBspec.seti [v1; v2] m)
   | enq_step3 vs m:
-      bq_step (bq_middlex enq vs m) E0 (bq_final Vundef m)
+      bq_step (bq_middle' enq vs m) E0 (bq_final Vundef m)
   | deq_step1 m:
       bq_step (bq_init deq [] m) E0 (bq_call RBspec.inc1 [] m)
   | deq_step2 v m:
       bq_step (bq_middle deq [v] m) E0 (bq_call RBspec.geti [v] m)
   | deq_step3 v m:
-      bq_step (bq_middlex deq v m) E0 (bq_final v m).
+      bq_step (bq_middle' deq v m) E0 (bq_final v m).
 
   Inductive bq_at_external: bq_internal_state -> c_query -> Prop :=
   | bq_ext_inc1 vf sig vs m b:
@@ -79,17 +79,17 @@ Section RB_LTS.
     bq_at_external (bq_call RBspec.seti vs m) (cq vf sig vs m).
 
   Inductive bq_after_external: bq_internal_state -> c_reply -> bq_internal_state -> Prop :=
-  | bq_aft_inc1 rv m :
+  | bq_aft_inc1 rv m m':
     Cop.val_casted rv tint ->
-    bq_after_external (bq_call RBspec.inc1 nil m) (cr rv m) (bq_middle deq [rv] m)
-  | bq_aft_inc2 rv v m :
+    bq_after_external (bq_call RBspec.inc1 nil m') (cr rv m) (bq_middle deq [rv] m)
+  | bq_aft_inc2 rv v m m':
     Cop.val_casted rv tint ->
-    bq_after_external (bq_call RBspec.inc2 [v] m) (cr rv m) (bq_middle enq [rv; v] m)
-  | bq_aft_get rv vs m :
+    bq_after_external (bq_call RBspec.inc2 [v] m') (cr rv m) (bq_middle enq [rv; v] m)
+  | bq_aft_get rv vs m m':
     Cop.val_casted rv tint ->
-    bq_after_external (bq_call RBspec.geti vs m) (cr rv m) (bq_middlex deq rv m)
-  | bq_aft_set vs m :
-    bq_after_external (bq_call RBspec.seti vs m) (cr Vundef m) (bq_middlex enq Vundef m).
+    bq_after_external (bq_call RBspec.geti vs m') (cr rv m) (bq_middle' deq rv m)
+  | bq_aft_set vs m m':
+    bq_after_external (bq_call RBspec.seti vs m') (cr Vundef m) (bq_middle' enq Vundef m).
 
   Program Definition bq_lts: lts li_c li_c bq_internal_state :=
     {|
@@ -111,19 +111,23 @@ Definition bq_spec: semantics li_c li_c :=
     footprint := AST.footprint_of_program bq_program;
   |}.
 
-Inductive bq_ms se: bq_internal_state -> Clight.state -> Prop :=
+Inductive bq_ms se: bq_internal_state * rb_state -> Clight.state -> Prop :=
 | bq_ms_enq:
-  forall vf m v,
+  forall vf m m' v srb,
     Cop.val_casted v tint ->
     Genv.find_funct (Genv.globalenv se bq_program) vf = Some (Internal bq_enq) ->
-    bq_ms se (bq_init enq [v] m) (Callstate vf [v] Kstop m)
+    rb_match_mem se srb m ->
+    Mem.nextblock m' = Mem.nextblock m ->
+    bq_ms se (bq_init enq [v] m', srb) (Callstate vf [v] Kstop m)
 | bq_ms_deq:
-  forall vf m,
+  forall vf m m' srb,
     Genv.find_funct (Genv.globalenv se bq_program) vf = Some (Internal bq_deq) ->
-    bq_ms se (bq_init deq [] m) (Callstate vf [] Kstop m)
+    rb_match_mem se srb m ->
+    Mem.nextblock m' = Mem.nextblock m ->
+    bq_ms se (bq_init deq [] m', srb) (Callstate vf [] Kstop m)
 
 | bq_ms_call_inc1:
-  forall vf k m b,
+  forall vf k m' m b srb,
     vf = Vptr b Integers.Ptrofs.zero ->
     Genv.find_symbol se inc1_id = Some b ->
     k = (Kcall (Some bq_deq_tmp1) bq_deq empty_env
@@ -132,9 +136,11 @@ Inductive bq_ms se: bq_internal_state -> Clight.state -> Prop :=
              (Ssequence
                 (Scall (Some bq_deq_tmp2) (Evar get_id (Tfunction (Tcons tint Tnil) tint cc_default))
                    [Etempvar bq_deq_tmp1 tint]) (Sreturn (Some (Etempvar bq_deq_tmp2 tint)))) Kstop)) ->
-    bq_ms se (bq_call RBspec.inc1 [] m) (Callstate vf [] k m)
+    rb_match_mem se srb m ->
+    Mem.nextblock m' = Mem.nextblock m ->
+    bq_ms se (bq_call RBspec.inc1 [] m', srb) (Callstate vf [] k m)
 | bq_ms_call_inc2:
-  forall vf k m v b,
+  forall vf k m m' v b srb,
     Cop.val_casted v tint ->
     vf = Vptr b Integers.Ptrofs.zero ->
     Genv.find_symbol se inc2_id = Some b ->
@@ -144,10 +150,12 @@ Inductive bq_ms se: bq_internal_state -> Clight.state -> Prop :=
              (Ssequence
                 (Scall None (Evar set_id (Tfunction (Tcons tint (Tcons tint Tnil)) tvoid cc_default))
                    [Etempvar bq_enq_tmp tint; Etempvar enq_arg_id tint]) (Sreturn None)) Kstop)) ->
-    bq_ms se (bq_call RBspec.inc2 [v] m) (Callstate vf [] k m)
+    rb_match_mem se srb m ->
+    Mem.nextblock m' = Mem.nextblock m ->
+    bq_ms se (bq_call RBspec.inc2 [v] m', srb) (Callstate vf [] k m)
 
 | bq_ms_mid_enq:
-  forall m v1 v2 k,
+  forall m m' v1 v2 k srb,
     Cop.val_casted v1 tint ->
     Cop.val_casted v2 tint ->
     k = (Kcall (Some bq_enq_tmp) bq_enq empty_env
@@ -156,9 +164,11 @@ Inductive bq_ms se: bq_internal_state -> Clight.state -> Prop :=
              (Ssequence
                 (Scall None (Evar set_id (Tfunction (Tcons tint (Tcons tint Tnil)) tvoid cc_default))
                    [Etempvar bq_enq_tmp tint; Etempvar enq_arg_id tint]) (Sreturn None)) Kstop)) ->
-    bq_ms se (bq_middle enq [v1; v2] m) (Returnstate v1 k m)
+    rb_match_mem se srb m ->
+    Mem.nextblock m' = Mem.nextblock m ->
+    bq_ms se (bq_middle enq [v1; v2] m', srb) (Returnstate v1 k m)
 | bq_ms_mid_deq:
-  forall m v k,
+  forall m m' v k srb,
     Cop.val_casted v tint ->
     k = (Kcall (Some bq_deq_tmp1) bq_deq empty_env
           (PTree.Node (PTree.Node PTree.Leaf (Some Vundef) PTree.Leaf) (Some Vundef) PTree.Leaf)
@@ -166,42 +176,54 @@ Inductive bq_ms se: bq_internal_state -> Clight.state -> Prop :=
              (Ssequence
                 (Scall (Some bq_deq_tmp2) (Evar get_id (Tfunction (Tcons tint Tnil) tint cc_default))
                    [Etempvar bq_deq_tmp1 tint]) (Sreturn (Some (Etempvar bq_deq_tmp2 tint)))) Kstop)) ->
-    bq_ms se (bq_middle deq [v] m) (Returnstate v k m)
+    rb_match_mem se srb m ->
+    Mem.nextblock m' = Mem.nextblock m ->
+    bq_ms se (bq_middle deq [v] m', srb) (Returnstate v k m)
 
 | bq_ms_call_get:
-  forall vf k m v b,
+  forall vf k m m' v b srb,
     vf = Vptr b Integers.Ptrofs.zero ->
     Genv.find_symbol se get_id = Some b ->
     Cop.val_casted v tint ->
     k = (Kcall (Some bq_deq_tmp2) bq_deq empty_env
           (PTree.Node (PTree.Node PTree.Leaf (Some Vundef) PTree.Leaf) (Some v) PTree.Leaf)
           (Kseq (Sreturn (Some (Etempvar bq_deq_tmp2 tint))) Kstop)) ->
-    bq_ms se (bq_call RBspec.geti [v] m) (Callstate vf [v] k m)
+    rb_match_mem se srb m ->
+    Mem.nextblock m' = Mem.nextblock m ->
+    bq_ms se (bq_call RBspec.geti [v] m', srb) (Callstate vf [v] k m)
 | bq_ms_call_set:
-  forall vf k m v1 v2 b,
+  forall vf k m m' v1 v2 b srb,
     vf = Vptr b Integers.Ptrofs.zero ->
     Genv.find_symbol se set_id = Some b ->
     Cop.val_casted v1 tint ->
     Cop.val_casted v2 tint ->
     k = (Kcall None bq_enq empty_env (PTree.Node (PTree.Node PTree.Leaf (Some v1) PTree.Leaf) (Some v2) PTree.Leaf) (Kseq (Sreturn None) Kstop)) ->
-    bq_ms se (bq_call RBspec.seti [v1; v2] m) (Callstate vf [v1; v2] k m)
+    rb_match_mem se srb m ->
+    Mem.nextblock m' = Mem.nextblock m ->
+    bq_ms se (bq_call RBspec.seti [v1; v2] m', srb) (Callstate vf [v1; v2] k m)
 
-| bq_ms_midx_enq:
-  forall m v k le,
+| bq_ms_mid'_enq:
+  forall m m' v k le srb,
     k = (Kcall None bq_enq empty_env le (Kseq (Sreturn None) Kstop)) ->
-    bq_ms se (bq_middlex enq v m) (Returnstate v k m)
-| bq_ms_midx_deq:
-  forall m v rv k,
+    rb_match_mem se srb m ->
+    Mem.nextblock m' = Mem.nextblock m ->
+    bq_ms se (bq_middle' enq v m', srb) (Returnstate v k m)
+| bq_ms_mid'_deq:
+  forall m m' v rv k srb,
     Cop.val_casted rv tint ->
     Cop.val_casted v tint ->
     k = (Kcall (Some bq_deq_tmp2) bq_deq empty_env
           (PTree.Node (PTree.Node PTree.Leaf (Some Vundef) PTree.Leaf) (Some v) PTree.Leaf)
           (Kseq (Sreturn (Some (Etempvar bq_deq_tmp2 tint))) Kstop)) ->
-    bq_ms se (bq_middlex deq rv m) (Returnstate rv k m)
+    rb_match_mem se srb m ->
+    Mem.nextblock m' = Mem.nextblock m ->
+    bq_ms se (bq_middle' deq rv m', srb) (Returnstate rv k m)
 
 | bq_ms_final:
-  forall rv m,
-    bq_ms se (bq_final rv m) (Returnstate rv Kstop m).
+  forall rv m m' srb,
+    rb_match_mem se srb m ->
+    Mem.nextblock m' = Mem.nextblock m ->
+    bq_ms se (bq_final rv m', srb) (Returnstate rv Kstop m).
 
 Import Ptrofs.
 
@@ -249,65 +271,70 @@ Opaque Genv.find_funct semantics2.
 Opaque semantics2.
 Opaque Nat.modulo.
 Require Import Lia.
+Opaque Genv.find_symbol.
 
-Lemma bq_correct: forward_simulation cc_id cc_id bq_spec (Clight.semantics2 bq_program).
+Lemma bq_correct': forward_simulation rb_cc rb_cc (bq_spec @ rb_state) (Clight.semantics2 bq_program).
 Proof.
   constructor. econstructor. reflexivity. firstorder.
   intros. instantiate (1 := fun _ _ _ => _). cbn beta.
   destruct H. subst.
-  set (ms := fun (s1: state bq_spec) s2 => bq_ms se1 s1 s2).
+  set (ms := fun (s1: state bq_spec * rb_state) s2 => bq_ms se2 s1 s2).
   eapply forward_simulation_plus with (match_states := ms).
-  - intros. destruct q1. inv H. inv H1.
+  - intros.  destruct q1, s1. inv H; inv H1; inv H; cbn in *; subst.
     + eexists. split.
       * econstructor; eauto.
         eapply genv_funct_symbol; eauto. reflexivity.
         unfold type_of_function. f_equal; cbn.
-        constructor; eauto. constructor.
+        constructor; eauto. constructor. rewrite H7. eauto.
       * constructor; eauto. eapply genv_funct_symbol; eauto.
     + eexists. split.
       * econstructor; eauto.
         eapply genv_funct_symbol; eauto. reflexivity.
         unfold type_of_function. f_equal; cbn.
-        constructor; eauto.
-      * constructor. eapply genv_funct_symbol; eauto.
-  - intros. destruct r1. inv H1. inv H.
-    eexists. split. constructor. constructor.
-  - intros. inv H1; inv H.
+        constructor; eauto. rewrite H7. eauto.
+      * constructor. eapply genv_funct_symbol; eauto. eauto. congruence.
+  - intros. destruct r1, s1. inv H1; inv H2. cbn in *. subst. inv H.
+    eexists. split. econstructor. constructor; eauto.
+  - intros. destruct s1, q1.  inv H1. inv H2; cbn in *; subst; inv H.
     (* inc1 *)
-    + eexists tt, _.  split. 2: split.
+    + eexists se2, _.  split. 2: split.
       * econstructor; eauto.
         eapply genv_funct_symbol; eauto. reflexivity.
       * assert (b = b0). cbn in *. congruence.
-        subst. constructor.
-      * split. constructor. intros. inv H. inv H1.
+        subst. constructor. eauto. congruence.
+      * split. eauto. intros.  destruct s1', r1, H1.
+        cbn in *. subst. inv H. inv H1.
         eexists. split; constructor; eauto.
     (* inc2 *)
-    + eexists tt, _.  split. 2: split.
+    + eexists se2, _.  split. 2: split.
       * econstructor; eauto.
         eapply genv_funct_symbol; eauto. reflexivity.
       * assert (b = b0).  cbn in *. congruence.
-        subst. constructor.
-      * split. constructor. intros. inv H. inv H1.
+        subst. constructor. eauto. congruence.
+      * split. eauto. intros. destruct s1', r1, H1.
+        cbn in *. subst. inv H. inv H1.
         eexists. split; constructor; eauto.
     (* get *)
-    + eexists tt, _.  split. 2: split.
+    + eexists se2, _.  split. 2: split.
       * econstructor; eauto.
         eapply genv_funct_symbol; eauto. reflexivity.
       * assert (b = b0). cbn in *. congruence.
-        subst. constructor.
-      * split. constructor. intros. inv H. inv H1.
+        subst. constructor. eauto. congruence.
+      * split. eauto. intros. destruct s1', r1, H1.
+        cbn in *. subst.  inv H. inv H1.
         eexists. split. econstructor; eauto.
-        econstructor. apply H8. apply H6. reflexivity.
+        econstructor. apply H13. apply H7. reflexivity. eauto. congruence.
     (* set *)
-    + eexists tt, _.  split. 2: split.
+    + eexists se2, _.  split. 2: split.
       * econstructor; eauto.
         eapply genv_funct_symbol; eauto. reflexivity.
       * assert (b = b0). cbn in *. congruence.
-        subst. constructor.
-      * split. constructor. intros. inv H. inv H1.
+        subst. constructor. eauto. congruence.
+      * split. eauto. intros. destruct s1', r1, H1.
+        cbn in *. subst. inv H. inv H1.
         eexists. split. econstructor; eauto.
-        econstructor. reflexivity.
-  - intros. inv H1; inv H.
+        econstructor. reflexivity. eauto. congruence.
+  - intros. destruct s1'.  inv H1; inv H; inv H1.
     (* enq: from initial to call inc2 *)
     + exploit inc2_block; eauto. intros (b1 & A & B).
       eexists. split.
@@ -353,13 +380,13 @@ Proof.
         lts_step. crush_step.
         lts_step. crush_step; crush_expr.
         apply star_refl. reflexivity.
-      * constructor.
+      * constructor; eauto.
     (* deq: to final state *)
     + eexists. split.
       * eapply plus_left. constructor.
         lts_step. crush_step.
         lts_step. crush_step; crush_expr.
         apply star_refl. reflexivity.
-      * constructor.
+      * constructor; eauto.
   - apply well_founded_ltof.
 Qed.
